disk-betree/PivotBetreeSpecRefinement.dfy
@@ -3,7 +3,7 @@ include "../lib/sequences.dfy"
 include "../lib/Maps.dfy"
 include "MapSpec.dfy"
 include "Graph.dfy"
-include "../tla-tree/MissingLibrary.dfy"
+include "../lib/Option.dfy"
 include "Message.dfy"
 include "BetreeSpec.dfy"
 include "Betree.dfy"
@@ -18,7 +18,7 @@ abstract module PivotBetreeSpecRefinement {
   import MS = MapSpec
   import opened Maps
   import opened Sequences
-  import opened MissingLibrary
+  import opened Options
   import opened PivotsLib
   import PivotBetreeSpecWFNodes
 
