lib/Option.dfy
@@ -1,0 +1,3 @@
+module Options {
+  datatype Option<V> = None | Some(value:V)
+} // module
