Makefile
@@ -1,4 +1,69 @@
+<<<<<<< HEAD
 ROOT=./
 TARGETS=
 
 include $(ROOT)/tools/Makefile.template
+=======
+#TARGETDLLS=a.dll b.dll
+#TARGETEXES=tttree.exe
+
+all: $(TARGETDLLS) $(TARGETEXES)
+
+DAFNY=dafny
+
+#####################################
+######## Automatic cleanups #########
+#####################################
+
+# Set this if you want make to remember what it builds so "make clean"
+# will work auto-magically.  You SHOULD NOT add this directory to
+# your version control system.
+BUILDINFO_DIR?=.build_info
+MD5SUM_PATH?=$(shell which md5sum md5 | head -1)
+
+ifdef BUILDINFO_DIR
+$(shell if [ ! -d $(BUILDINFO_DIR) ]; then mkdir $(BUILDINFO_DIR); fi)
+record_build=$(shell echo $(1) > $(BUILDINFO_DIR)/`echo $(1) | $(MD5SUM_PATH) | cut -f1 -d" "`)
+buildinfo_files=$(wildcard $(BUILDINFO_DIR)/*)
+else
+record_build=$(shell exit 0)
+endif
+
+clean:
+ifdef BUILDINFO_DIR
+	for i in $(buildinfo_files); do rm `cat $$i`; done
+	rm -rf $(BUILDINFO_DIR)
+endif
+
+###############################################
+######## Automatic dafny dependencies #########
+###############################################
+
+include $(TARGETDLLS:.dll=.deps) $(TARGETEXES:.exe=.deps)
+
+%.deps: %.dfy
+	$(DAFNY) /printIncludes:Transitive $< | grep ";" | grep -v "^roots;" | sed "s/\(^[^;]*\);/\1: /" | sed "s/;/ /g" | sed "s/.dfy/.dll/g" | sed "s,$(PWD)/,,g" > $@
+	$(DAFNY) /printIncludes:Transitive $< | grep -v ";" | sed "s,$(PWD)/,,g" | sed "s,^,$@: ," >> $@
+	$(call record_build, $@)
+
+############################################
+######## Generic dafny build rules #########
+############################################
+
+%.exe: %.dfy
+	$(DAFNY) $<
+	$(call record_build, $@)
+	$(call record_build, $@.mdb)
+
+%.dll: %.dfy 
+	$(DAFNY) $<
+	$(call record_build, $@)
+	$(call record_build, $@.mdb)
+
+build/Bundle.cs: $(shell find . -name '*.dfy')
+	mkdir -p build
+	dafny disk-betree/Bundle.dfy /spillTargetCode:3 /noVerify /compile:0 /out:build/Bundle.cs /countVerificationErrors:0
+
+build/Veribetrfs.exe: disk-betree/Framework.cs build/Bundle.cs
+	csc build/Bundle.cs disk-betree/Framework.cs /r:System.Numerics.dll /debug /nowarn:0164 /nowarn:0219 /nowarn:1717 /nowarn:0162 /nowarn:0168 /out:build/Veribetrfs.exe
+>>>>>>> Makefile rule for Veribetrfs.exe
